\documentclass[12pt]{article}
\usepackage[utf8]{inputenc}
\usepackage{amsmath}

\title{Chapter 7.1 Basic Integration Rules}
\author{Fritz Adelbertus Sitindaon}
\date{13 December 2022}

\begin{document}
\maketitle

\section{Perform the Indicated Integrations!}  
  
\begin{enumerate}
\item $\displaystyle\int(x-2)^5 \ dx $

Let $u = x-2$ and $du = dx$
\begin{equation*}
\begin{aligned}
\int(x-2)^5 \ dx &= \int u^5 \ du \\
&= \frac{1}{6}u^6 + C \\
&= \frac{1}{6}(x-2)^6 + C
\end{aligned}
\end{equation*}

\item $\displaystyle\int\sqrt{3x} \ dx $

Let $u = 3x$ and $du = 3dx$
\begin{equation*}
\begin{aligned}
\int \sqrt{3x} \ dx &= \int \sqrt{3x}\ \frac{3}{3} \ dx \\
&= \frac{1}{3} \int \sqrt{u} \, du \\
&= \frac{1}{3} \ \frac{2}{3} u^{3/2} + C \\
&= \frac{2}{9} (3x)^{3/2} + C
\end{aligned}
\end{equation*}
  
\item $\displaystyle\int_0^2x(x^2+1)^5 \ dx $

Let $u = x^2+1$ and $du = 2x\,dx$ \\
Let the upper limit = 5 and the lower limit = 1 
\begin{equation*}
\begin{aligned}
\int_0^2x(x^2+1)^5 \ dx  &= \frac{1}{2} \int_0^2(x^2+1)^5 \ 2x\,dx \\
&= \frac{1}{2} \int_1^5 u^5 \ du \\
&= \frac{1}{2} \ \left[\frac{1}{6} u^6\right]_1^5 \\
&= \frac{1}{2} \left(\frac{1}{6} 5^6 - \frac{1}{6} 1^6 \right) \\
&= \frac{1}{2} (2604) \\
&= 1302
\end{aligned}
\end{equation*}

\item $\displaystyle\int_0^1x\sqrt{1-x^2} \ dx $

Let $u = 1-x^2$ and $du = -2x\,dx$ \\
Let the upper limit = 0 and the lower limit = 1 
\begin{equation*}
\begin{aligned}
\int_0^1x\sqrt{1-x^2} \ dx  &= -\frac{1}{2} \int_0^1\sqrt{1-x^2} \ -2x\,dx \\
&= -\frac{1}{2} \int_1^0\sqrt{u} \ du \\
&= \frac{1}{2} \int_0^1\sqrt{u} \ du \\
&= \frac{1}{2} \ \left[\frac{2}{3} u^{3/2}\right]_0^1 \\
&= \frac{1}{2} \left(\frac{2}{3} 1^{3/2} - \frac{2}{3} 0^{3/2} \right) \\
&= \frac{1}{2} \ \frac{2}{3} \\
&= \frac{1}{3}
\end{aligned}
\end{equation*}

\item $\displaystyle\int \frac{dx}{x^2+4}$

Remember $\int\frac{1}{a^2+x^2}dx = \frac{1}{a}\arctan\left(\frac{x}{a}\right)$
\begin{equation*}
\begin{aligned}
\int \frac{dx}{x^2+4} &= \int \frac{1}{2^2+x^2} \ dx \\
&=\frac{1}{2}\arctan\left(\frac{x}{2}\right) + C
\end{aligned}
\end{equation*}

\item $\displaystyle\int \frac{e^x}{2+e^x} \ dx$

Let $u = 2+e^x$ and $du = e^x\,dx$
\begin{equation*}
\begin{aligned}
\int \frac{e^x}{2+e^x} \ dx &= \int \frac{1}{2+e^x} \ e^x dx \\
&= \int \frac{1}{u} \ du \\
&= ln|u| + C \\
&= ln|2+e^x| + C \\
&= ln(2+e^x) + C
\end{aligned}
\end{equation*}

\item $\displaystyle\int \frac{x}{x^2+4} \ dx$

Let $u = x^2+4$ and $du = 2x\,dx$
\begin{equation*}
\begin{aligned}
\int \frac{x}{x^2 + 4} \ dx &= \frac{1}{2}\int \frac{1}{x^2+4} \ 2x\,dx \\
&= \frac{1}{2}\int \frac{1}{u} \ du \\
&= \frac{1}{2} ln|u| + C \\
&= \frac{1}{2} ln|x^2+4| + C \\
&= \frac{1}{2} ln(x^2+4) + C
\end{aligned}
\end{equation*}

\item $\displaystyle\int \frac{2t^2}{2t^2+1} \ dt$

Let $u = \sqrt{2}t$ and $du = \sqrt{2}\,dt$
\begin{equation*}
\begin{aligned}
\int \frac{2t^2}{2t^2 + 1} \ dt &= \int \frac{2t^2+1-1}{2t^2+1} \ dt \\
&= \int \frac{2t^2+1}{2t^2+1}-\frac{1}{2t^2+1} \ dt \\
&= \int dt -\int\frac{1}{2t^2+1} \ dt \\
&= t - \int \frac{1}{1^2 + (\sqrt{2}t)^2} \ dt\\
&= t - \frac{1}{\sqrt{2}}\int \frac{1}{1^2 + (\sqrt{2}t)^2} \ \sqrt{2}t\,dt\\
&= t - \frac{1}{\sqrt{2}}\int \frac{1}{1^2 + u^2} \ du\\
&= t - \frac{1}{\sqrt{2}}\arctan u + C\\
&= t - \frac{1}{\sqrt{2}}\arctan(\sqrt{2}t) + C\\
\end{aligned}
\end{equation*}

\item $\displaystyle\int 6z \sqrt{4+z^2} \ dz$

Let $u = 4+z^2$ and $du = 2z\,dz$
\begin{equation*}
\begin{aligned}
\int 6z \sqrt{4+z^2} \ dz &= 3\int \sqrt{4+z^2} \ 2z\,dz \\
&= 3\int \sqrt{u} \ du \\
&= 3\,\frac{2}{3} u^{3/2} + C \\
&= 2 (4+z^2)^{3/2} + C
\end{aligned}
\end{equation*}

\item $\displaystyle\int \frac{5}{\sqrt{2t+1}} \ dt$

Let $u = 2t+1$ and $du = 2\,dt$
\begin{equation*}
\begin{aligned}
\int \frac{5}{\sqrt{2t+1}} \ dt &= \frac{5}{2}\int\frac{1}{\sqrt{2t+1}} \ 2\,dt \\
&= \frac{5}{2}\int\frac{1}{\sqrt{u}} \ du \\
&= \frac{5}{2}2u^{1/2}+ C \\
&= 5\sqrt{2t+1} + C
\end{aligned}
\end{equation*}
\end{enumerate}

\end{document}
