\documentclass[12pt]{article}
\usepackage[utf8]{inputenc}
\usepackage{amsmath}
\usepackage[a4paper, total={20cm, 25cm}]{geometry}
\usepackage{tikz}
\usepackage{multicol}

\title{Chapter 7.4 Rationalizing Subtitutions}
\author{Fritz Adelbertus Sitindaon}
\date{15 December 2022}

\begin{document}
\maketitle

\section{Perform the Indicated Integrations!}  
  
\begin{enumerate}
%Number 1
\item $\displaystyle\int x\sqrt{x+1}\,dx$

Let $u=\sqrt{x+1}$, $x=u^{2}-1$ and $dx=2u\,du$
\begin{equation*}
  \begin{aligned}
  \int x\sqrt{x+1}\,dx &= \int (u^{2}-1)(u)2u\,du\\
  &=\int 2u^{4}-2u^{2}\,du\\
  &=\frac{2}{5}u^{5}-\frac{2}{3}u^{3}+C\\
  &=\frac{2}{5}(x+1)^{5/2}-\frac{2}{3}(x+1)^{3/2}+C
  \end{aligned}
\end{equation*}

%Number 2
\item $\displaystyle\int x\sqrt[3]{x+\pi}\,dx$

Let $u=\sqrt[3]{x+\pi}$, $x=u^{3}-\pi$ and $dx=3u^{2}\,du$
\begin{equation*}
  \begin{aligned}
  \int x\sqrt[3]{x+\pi}\,dx &= \int(u^{3}-\pi)(u)3u^{2}\,du\\
  &=\int 3u^{6}-3\pi u^{3}\,du\\
  &=\frac{3}{7}u^{7}-\frac{3\pi}{4}u^{4}+C\\
  &=\frac{3}{7}(x+\pi)^{7/3}-\frac{3\pi}{4}(x+\pi)^{4/3}+C
  \end{aligned}
\end{equation*}

%Number 3
\item $\displaystyle\int\frac{t\,dt}{\sqrt{3t+4}}$

Let $u=\sqrt{3t+4}$, $t=\displaystyle\frac{u^{2}-4}{3}$ and $dt=\displaystyle\frac{2}{3}u\,du$
\begin{equation*}
  \begin{aligned}
  \int\frac{t\,dt}{\sqrt{3t+4}} &= \int\frac{u^{2}-4}{3}\,\frac{1}{u}\,\frac{2}{3}u\,du\\
  &=\int\frac{2}{9}u^{2}-\frac{8}{9}\,du\\
  &=\frac{2}{27}u^{3}-\frac{8}{9}u+C\\
  &=\frac{2}{27}(3t+4)^{3/2}-\frac{8}{9}(3t+4)^{1/2}+C
  \end{aligned}
\end{equation*}

%Number 4
\item $\displaystyle\int\frac{x^{2}+3x}{\sqrt{x+4}}\,dx$

Let $u=\sqrt{x+4}$, $x=u^{2}-4$ and $dx=2u\,du$
\begin{equation*}
  \begin{aligned}
  \int\frac{x^{2}+3x}{\sqrt{x+4}}\,dx &= \int\frac{(u^{2}-4)^{2}+3(u^{2}-4)}{u}\,2u\,du\\
  &=2\int(u^{4}-8u^{2}+16)+3u^{2}-12\,du\\
  &=2\int u^{4}-5u^{2}+4\,du\\
  &=2\left(\frac{1}{5}u^{5}-\frac{5}{3}u^{3}+4u\right)+C\\
  &=\frac{2}{5}(x+4)^{5/2}-\frac{10}{3}(x+4)^{3/2}+8(x+4)^{1/2}+C
  \end{aligned}
\end{equation*}

%Number 5
\item $\displaystyle\int_1^2\frac{dt}{\sqrt{t}+e}$

Let $u=\sqrt{t}+e$, $t=(u-e)^{2}$ and $dt=2u-2e\,du$
\begin{equation*}
  \begin{aligned}
  \int\frac{dt}{\sqrt{t}+e} &= \int\frac{1}{u}(2u-2e)\,du\\
  &=\int 2-\frac{2e}{u}\,du\\
  &=2u-2e\ln u+C\\
  &=2\sqrt{t}+2e-2e\ln(\sqrt{t}+e)+C\\
  \int_1^2\frac{dt}{\sqrt{t}+e} &= \left[2\sqrt{t}+2e-2e\ln(\sqrt{t}+e)\right]_1^2\\
  &=(2\sqrt{2}+2e-2e\ln(\sqrt{2}+e))-(2\sqrt{1}+2e-2e\ln(\sqrt{1}+e))\\
  &=2\sqrt{2}-2-2e\ln(\sqrt{2}+e)+2e\ln(1+e)\\
  &=2\sqrt{2}-2-2e\ln\left(\frac{\sqrt{2}+e}{1+e}\right)
  \end{aligned}
\end{equation*}

%Number 6
\item $\displaystyle\int_0^1\frac{\sqrt{t}}{t+1}\,dt$

Let $u=\sqrt{t}$, $t=u^{2}$ and $dt=2u\,du$
\begin{equation*}
  \begin{aligned}
  \int\frac{\sqrt{t}}{t+1}\,dt &=\int\frac{u}{u^{2}+1}\,2u\,du\\
  &=2\int\frac{u^{2}}{u^{2}+1}\,du\\
  &=2\int\frac{u^{2}+1-1}{u^{2}+1}\,du\\
  &=2\int\frac{u^{2}+1}{u^{2}+1}-\frac{1}{u^{2}+1}\,du\\
  &=2\int du - 2\int\frac{1}{u^{2}+1}\,du\\
  &=2u - 2\arctan u + C \\
  &=2\sqrt{t} - 2\arctan\sqrt{t} + C \\
  \int_0^1\frac{\sqrt{t}}{t+1}\,dt &=\left[2\sqrt{t} - 2\arctan\sqrt{t}\right]_0^1\\
  &=\left(2\sqrt{1} - 2\arctan\sqrt{1}\right)-\left(2\sqrt{0} - 2\arctan\sqrt{0}\right)\\
  &=2-\frac{\pi}{2}\\
  &\approx 0.4292
  \end{aligned}
\end{equation*}

%Number 7
\item $\displaystyle\int t(3t+2)^{3/2}\,dt$

Let $u=(3t+2)^{3/2}$, $t=\displaystyle\frac{u^{2/3}-2}{3}$ and $dt=\displaystyle\frac{2}{9}u^{-1/3}\,du$
\begin{equation*}
  \begin{aligned}
  \int t(3t+2)^{3/2}\,dt&=\int\frac{u^{2/3}-2}{3}(u)\frac{2}{9}u^{-1/3}\,du\\
  &=\int\frac{2}{27}u^{4/3}-\frac{4}{27}u^{2/3}\,du\\
  &=\frac{2}{63}u^{7/3}-\frac{4}{45}u^{5/3}+C\\
  &=\frac{2}{63}(3t+2)^{7/2}-\frac{4}{45}u^{5/2}+C
  \end{aligned}
\end{equation*}

%Number 8
\item $\displaystyle\int x(1-x)^{2/3}\,dx$

Let $u=(1-x)^{2/3}$, $x=1-u^{3/2}$ and $dx=\displaystyle-\frac{3}{2}u^{1/2}\,du$
\begin{equation*}
  \begin{aligned}
  \int x(1-x)^{2/3}\,dx &=\int(1-u^{3/2})(u)\left(-\frac{3}{2}u^{1/2}\right)du\\
  &=-\frac{3}{2}\int u^{3/2}-u^{3}\,du\\
  &=-\frac{3}{2}\left(\frac{2}{5}u^{5/2}-\frac{1}{4}u^{4}\right)+C\\
  &=\frac{3}{8}(1-x)^{8/3}-\frac{3}{5}(1-x)^{5/3}+C
  \end{aligned}
\end{equation*}





%Number 9
\begin{multicols}{2}
  \item $\displaystyle\int\frac{\sqrt{4-x^{2}}}{x}\,dx$

  Let $x=2\sin u$ and $dx=2\cos u\,du$\\
  Using the triangle, we obtained these values:
  
  $\cos u=\displaystyle\frac{\sqrt{4-x^{2}}}{2}$,
  $\csc u=\displaystyle\frac{2}{x}$,
  $\cot u=\displaystyle\frac{\sqrt{4-x^{2}}}{x}$
  \break
  \begin{tikzpicture}
    \draw (0,0)--(4,0) node[pos=0.5, below]{$\sqrt{4-x^{2}}$};
    \draw (4,0)--(4,3) node[pos=0.5, right]{$x$};
    \draw (4,3)--(0,0) node[pos=0.5, above, rotate=37]{$2$};
  \end{tikzpicture}
\end{multicols}
\begin{equation*}
  \begin{aligned}
  \int\frac{\sqrt{4-x^{2}}}{x}\,dx &=\int\frac{\sqrt{4-(2\sin u)^{2}}}{2\sin u}\,2\cos u\,du\\
  &=\int\frac{\sqrt{4-(4\sin^{2}u)}}{\sin u}\,\cos u\,du\\
  &=\int\frac{2\sqrt{1-\sin^{2}u}}{\sin u}\,\cos u\,du\\
  &=2\int\frac{\cos u}{\sin u}\,\cos u\,du\\
  &=2\int\frac{\cos^{2}u}{\sin u}\,du\\
  &=2\int\frac{1-\sin^{2}u}{\sin u}\,du\\
  &=2\int\frac{1}{\sin u}-\frac{\sin^{2}u}{\sin u}\,du\\
  &=2\int\csc\,du-2\int\sin u\,du\\
  &=2\ln|\csc u-\cot u|+2\cos u + C\\
  &=2\ln\left|\frac{2}{x}-\frac{\sqrt{4-x^{2}}}{x}\right|+2\frac{\sqrt{4-x^{2}}}{2}+C\\
  &=2\ln\left|\frac{2-\sqrt{4-x^{2}}}{x}\right|+\sqrt{4-x^{2}}+C
  \end{aligned}
\end{equation*}

%Number 10
\begin{multicols}{2}
  \item $\displaystyle\int\frac{x^{2}dx}{\sqrt{16-x^{2}}}$
  
  Let $x=4\sin u$, $dx=4\cos u\,du$, and $\displaystyle u=\arcsin\left(\frac{x}{4}\right)$\\
  Using the triangle, we obtained the values below:
  
  $\cos u=\displaystyle\frac{\sqrt{16-x^{2}}}{2}$\\\break
  \begin{tikzpicture}
    \draw (0,0)--(4,0) node[pos=0.5, below]{$\sqrt{16-x^{2}}$};
    \draw (4,0)--(4,3) node[pos=0.5, right]{$x$};
    \draw (4,3)--(0,0) node[pos=0.5, above, rotate=37]{$4$};
  \end{tikzpicture}
\end{multicols}
\begin{equation}
  \begin{aligned}
  \int\frac{x^{2}dx}{\sqrt{16-x^{2}}}&=\int\frac{(4\sin u)^{2}}{\sqrt{16-(4\sin u)^{2}}}\,4\cos u\,dx\\
  &=4\int\frac{16\sin^{2}u}{\sqrt{16-16\sin^{2}u}}\,\cos u\,du\\
  &=64\int\frac{\sin^{2}u}{4\sqrt{1-\sin^{2}u}}\,\cos u\,du\\
  &=16\int\frac{\sin^{2}u}{\cos u}\,\cos u\,du\\
  &=16\int\sin^{2}u\,du\\  
  \end{aligned}
\end{equation}
Evaluate $\displaystyle\int\sin^{2}u\,du$
\begin{equation}
  \begin{aligned}
  \int\sin^{2}u\,du&=\int\frac{1-\cos{2u}}{2}\,du\\
  &=\frac{1}{2}\int\,du-\frac{1}{2}\int\cos{2u}\,du\\
  &=\frac{1}{2}u-\frac{1}{4}\sin{2u}+C
  \end{aligned}
\end{equation}
Subtitue back to the original problem
\begin{equation}
  \begin{aligned}
  \int\frac{x^{2}dx}{\sqrt{16-x^{2}}}&=16\int\sin^{2}u\,du\\
  &=16\left(\frac{1}{2}u-\frac{1}{4}\sin{2u}\right)+C\\
  &=8u-4\sin{2u}+C\\
  &=8u-8\sin{u}\cos{u}+C\\
  &=8\arcsin\left(\frac{x}{4}\right)-8\left(\frac{x}{4}\,\frac{\sqrt{16-x^{2}}}{4}\right)+C\\
  &=8\arcsin\left(\frac{x}{4}\right)-\frac{x\sqrt{16-x^{2}}}{2}+C
  \end{aligned}
\end{equation}
\end{enumerate}

\end{document}
