\documentclass[12pt]{article}
\usepackage[utf8]{inputenc}
\usepackage{amsmath}
\usepackage[a4paper, total={20cm, 25cm}]{geometry}
\usepackage{tikz}
\usepackage{multicol}

\title{Chapter 6.9 The Hyperbolic Functions and Their Inverses}
\author{Fritz Adelbertus Sitindaon}
\date{22 December 2022}

\begin{document}
\maketitle

\section{Verify the Identities for the given equations!}  
  
\begin{enumerate}
%Number 1
\item $\displaystyle e^x = \cosh x+\sinh x$

\begin{equation*}
  \begin{aligned}
  e^x &= \cosh x+\sinh x\\
  &=\frac{e^x+e^{-x}}{2}+\frac{e^x-e^{-x}}{2}\\
  &=\frac{2e^x}{2}\\
  &=e^x
  \end{aligned}
\end{equation*}

%Number 2
\item $\displaystyle e^{2x} = \cosh2x+\sinh2x$

\begin{equation*}
  \begin{aligned}
  e^{2x} &= \cosh2x+\sinh2x\\
  &=\frac{e^{2x}+e^{-2x}}{2}+\frac{e^{2x}-e^{-2x}}{2}\\
  &=\frac{2e^{2x}}{2}\\
  &=e^{2x}
  \end{aligned}
\end{equation*}

%Number 3
\item $\displaystyle e^x = \cosh x-\sinh x$

\begin{equation*}
  \begin{aligned}
  e^{-x} &= \cosh x+\sinh x\\
  &=\frac{e^x+e^{-x}}{2}-\frac{e^x-e^{-x}}{2}\\
  &=\frac{2e^{-x}}{2}\\
  &=e^{-x}
  \end{aligned}
\end{equation*}

%Number 4
\item $\displaystyle e^{2x} = \cosh2x-\sinh2x$

\begin{equation*}
  \begin{aligned}
  e^{-2x} &= \cosh2x-\sinh2x\\
  &=\frac{e^{2x}+e^{-2x}}{2}-\frac{e^{2x}-e^{-2x}}{2}\\
  &=\frac{2e^{-2x}}{2}\\
  &=e^{-2x}
  \end{aligned}
\end{equation*}

%Number 5
\item $\displaystyle\sinh(x+y)=\sinh{x}\cosh{y}+\cosh{x}\sinh{x}$

\begin{equation*}
  \begin{aligned}
  \sinh(x+y)&=\sinh{x}\cosh{y}+\cosh{x}\sinh{x}\\
  &=\frac{e^x-e^{-x}}{2}\times\frac{e^y+e^{-y}}{2}+\frac{e^x+e^{-x}}{2}\times\frac{e^y-e^{-y}}{2}\\
  &=\frac{e^{x+y}+e^{x-y}-e^{-x+y}-e^{-x-y}}{4}+\frac{e^{x+y}-e^{x-y}+e^{-x+y}-e^{-x-y}}{4}\\
  &=\frac{2e^{x+y}-2e^{-x-y}}{4}\\
  &=\frac{e^{x+y}-e^{-(x+y)}}{2}\\
  &=\sinh(x+y)
  \end{aligned}
\end{equation*}

%Number 6
\item $\displaystyle\sinh(x-y)=\sinh{x}\cosh{y}-\cosh{x}\sinh{x}$

\begin{equation*}
  \begin{aligned}
  \sinh(x-y)&=\sinh{x}\cosh{y}-\cosh{x}\sinh{x}\\
  &=\frac{e^x-e^{-x}}{2}\times\frac{e^y+e^{-y}}{2}-\frac{e^x+e^{-x}}{2}\times\frac{e^y-e^{-y}}{2}\\
  &=\frac{e^{x+y}+e^{x-y}-e^{-x+y}-e^{-x-y}}{4}-\frac{e^{x+y}-e^{x-y}+e^{-x+y}-e^{-x-y}}{4}\\
  &=\frac{2e^{x-y}-2e^{-x+y}}{4}\\
  &=\frac{e^{x-y}-e^{-(x-y)}}{2}\\
  &=\sinh(x-y)
  \end{aligned}
\end{equation*}

%Number 7
\item $\displaystyle\cosh(x+y)=\cosh{x}\cosh{y}+\sinh{x}\sinh{y}$

\begin{equation*}
  \begin{aligned}
  \cosh(x+y)&=\cosh{x}\cosh{y}+\sinh{x}\sinh{y}\\
  &=\frac{e^x+e^{-x}}{2}\times\frac{e^y+e^{-y}}{2}+\frac{e^x-e^{-x}}{2}\times\frac{e^y-e^{-y}}{2}\\
  &=\frac{e^{x+y}+e^{x-y}+e^{-x+y}+e^{-x-y}}{4}+\frac{e^{x+y}-e^{x-y}-e^{-x+y}+e^{-x-y}}{4}\\
  &=\frac{2e^{x+y}+2e^{-x-y}}{4}\\
  &=\frac{e^{x+y}+e^{-(x+y)}}{2}\\
  &=\cosh(x+y)
  \end{aligned}
\end{equation*}

%Number 8
\item $\displaystyle\cosh(x-y)=\cosh{x}\cosh{y}-\sinh{x}\sinh{y}$

\begin{equation*}
  \begin{aligned}
  \cosh(x-y)&=\cosh{x}\cosh{y}-\sinh{x}\sinh{y}\\
  &=\frac{e^x+e^{-x}}{2}\times\frac{e^y+e^{-y}}{2}-\frac{e^x-e^{-x}}{2}\times\frac{e^y-e^{-y}}{2}\\
  &=\frac{e^{x+y}+e^{x-y}+e^{-x+y}+e^{-x-y}}{4}-\frac{e^{x+y}-e^{x-y}-e^{-x+y}+e^{-x-y}}{4}\\
  &=\frac{2e^{x-y}+2e^{-x+y}}{4}\\
  &=\frac{e^{x-y}+e^{-(x-y)}}{2}\\
  &=\cosh(x-y)
  \end{aligned}
\end{equation*}

%Number 9
\item $\displaystyle\tanh(x+y)=\frac{\tanh{x}+\tanh{y}}{1+\tanh{x}\tanh{y}}$

\begin{equation*}
  \begin{aligned}
  \tanh(x+y)&=\frac{\tanh{x}+\tanh{y}}{1+\tanh{x}\tanh{y}}\\
  &=\frac{\frac{\sinh{x}}{\cosh{x}}+\frac{\sinh{y}}{\cosh{y}}}{1+\frac{\sinh{x}}{\cosh{x}}\times\frac{\sinh{y}}{\cosh{y}}}\\
  &=\frac{\frac{\sinh{x}\cosh{y}+\cosh{x}\sinh{y}}{\cosh{x}\cosh{y}}}{1+\frac{\sinh{x}\sinh{y}}{\cosh{x}\cosh{y}}}\\
  &=\frac{\frac{\sinh{x}\cosh{y}+\cosh{x}\sinh{y}}{\cosh{x}\cosh{y}}}{\frac{\cosh{x}\cosh{y}+\sinh{x}\sinh{y}}{\cosh{x}\cosh{y}}}\\
  &=\frac{\sinh{x}\cosh{y}+\cosh{x}\sinh{y}}{\cosh{x}\cosh{y}+\sinh{x}\sinh{y}}\\
  &=\frac{\sinh(x+y)}{\cosh(x+y)}\\
  &=\tanh(x+y)
  \end{aligned}
\end{equation*}

%Number 10
\item $\displaystyle\tanh(x-y)=\frac{\tanh{x}-\tanh{y}}{1-\tanh{x}\tanh{y}}$

\begin{equation*}
  \begin{aligned}
  \tanh(x-y)&=\frac{\tanh{x}-\tanh{y}}{1-\tanh{x}\tanh{y}}\\
  &=\frac{\frac{\sinh{x}}{\cosh{x}}-\frac{\sinh{y}}{\cosh{y}}}{1-\frac{\sinh{x}}{\cosh{x}}\times\frac{\sinh{y}}{\cosh{y}}}\\
  &=\frac{\frac{\sinh{x}\cosh{y}-\cosh{x}\sinh{y}}{\cosh{x}\cosh{y}}}{1-\frac{\sinh{x}\sinh{y}}{\cosh{x}\cosh{y}}}\\
  &=\frac{\frac{\sinh{x}\cosh{y}-\cosh{x}\sinh{y}}{\cosh{x}\cosh{y}}}{\frac{\cosh{x}\cosh{y}-\sinh{x}\sinh{y}}{\cosh{x}\cosh{y}}}\\
  &=\frac{\sinh{x}\cosh{y}-\cosh{x}\sinh{y}}{\cosh{x}\cosh{y}-\sinh{x}\sinh{y}}\\
  &=\frac{\sinh(x-y)}{\cosh(x-y)}\\
  &=\tanh(x-y)
  \end{aligned}
\end{equation*}
\end{enumerate}

\end{document}
